For debugging PopTLQD

src/Queue.v
@@ -2,7 +2,7 @@
 From Coq Require Import Arith List Psatz Morphisms Relations.
 From Equations Require Import Equations.
 
-From Clairvoyance Require Import Core Approx ApproxM Tick Misc ListA QueueInterface QueueTrace.
+From Clairvoyance Require Import Core Approx ApproxM Tick Misc List ListA QueueInterface QueueTrace BankersQueue.
 
 #[local] Existing Instance Exact_id | 1.
 #[local] Existing Instance LessDefined_id | 100.
@@ -22,7 +22,7 @@ Proof.
   unfold Proper, respectful. lia.
 Qed.
 
-(* ---------------------- Queue operations ---------------------- *)
+(** Queue implementation! **)
 
 Record two_list_queue (a : Type) : Type := TwoListQueue
 {
@@ -30,10 +30,27 @@ Record two_list_queue (a : Type) : Type := TwoListQueue
   QueueBack : list a
 }.
 
+Record two_list_queueA (a : Type) : Type := TwoListQueueA
+{
+  QueueFrontA : T (listA a);
+  QueueBackA : T (listA a)
+}.
+
+Global Instance Exact_two_list_queue {a b} {e : Exact a b} : Exact (two_list_queue a) (two_list_queueA b) :=
+  fun queue => match queue with
+    | TwoListQueue front back => TwoListQueueA (exact front) (exact back)
+    end.
+
 Definition Push_TwoListQueue (a : Type) (queue : two_list_queue a) (appending : a) : two_list_queue a :=
-  let back := appending :: QueueBack queue in
+  let old_back := QueueBack queue in
+  let new_back := appending :: old_back in
   let front := QueueFront queue in
-  TwoListQueue front back.
+  TwoListQueue front new_back.
+
+Definition Push_TwoListQueueD (a : Type) (queue : two_list_queue a) (appending : a) (outD : two_list_queueA a) :
+  Tick (T (two_list_queueA a) * T a) :=
+  Tick.tick >>
+  Tick.ret ((Thunk (TwoListQueueA (QueueFrontA outD) (tailX (QueueBackA outD)))), Thunk appending).
 
 Definition SwapBack (a : Type) (queue : two_list_queue a) : (two_list_queue a) :=
   match QueueFront queue with
@@ -48,36 +65,43 @@ Definition Pop_TwoListQueue (a : Type) (queue : two_list_queue a) : ((option a) 
   | x :: xs => (Some x, TwoListQueue xs (QueueBack new_queue))
   end.
 
-Record two_list_queueA (a : Type) : Type := TwoListQueueA
-{
-  QueueFrontA : T (listA a);
-  QueueBackA : T (listA a)
-}.
+(*Borrowed from Banker's Queue in large part.*)
 
-Definition Push_TwoListQueueD (a : Type) (queue : two_list_queue a) (appending : a)
-  (outD : two_list_queueA a) : Tick (T (two_list_queueA a)) :=
+(*Quoted from there...*)
+
+(* "[mkQueue] uses [rev] and [append], in this order ([append front (rev back)]),
+   so we compute the demand in reverse." *)
+
+Definition SwapBackD {a} (queue : two_list_queue a) (outD : (option (T a) * T (two_list_queueA a))) :
+  Tick (T (two_list_queueA a)) :=
   Tick.tick >>
-  match (QueueBackA outD) with
-  | Undefined => bottom
-  | Thunk xsD => match xsD with
-    | NilA => bottom
-    | ConsA yD ysD => Tick.ret (Thunk (TwoListQueueA (QueueFrontA outD) (exact (ConsA yD ysD))))
-  end
-end.
-
-(** Unfinished Pop_TwoListQueueD implementation **)
-
-(* Definition Pop_TwoListQueueD (a : Type) (queue : two_list_queue a)
-  (outD : (two_list_queueA a) * a) : Tick (T (two_list_queueA a)) :=
-  Tick.tick >>
-  match outD (*Need to access queuefront of outD's first element*) with
-  | (Undefined, _, _) => bottom
-  | (_, Undefined, _) => bottom
-  | (Thunk xsD, Thunk ysD, popped) => match xsD with
-    | NilA => bottom
-    | ConsA yD ysD => Tick.ret (Thunk outD)
+  match QueueFront queue with
+  | nil => match QueueBack queue with
+    | nil => Tick.ret (exact queue)
+    (*Non-empty case - undo the swap*)
+    | h :: t => match outD with
+      | (Some (xA, queueA)) =>
+        let+ (frontD, rbackD) := thunkD (appendD (QueueFront queue) (rev (QueueBack queue))) (QueueFrontA queueA) in
+        let+ backD := thunkD (revD (QueueBack queue)) rbackD in
+        Tick.ret (Thunk (TwoListQueueA frontD backD))
+      | _ => bottom
+      end
     end
-  end. *)
+  | _ => Tick.ret (exact queue)
+  end.
+
+Definition Pop_TwoListQueueD (a : Type) (queue : two_list_queue a) (outD : ((option (T a)) * (T (two_list_queueA a)))) :
+  Tick (T (two_list_queueA a)) :=
+  Tick.tick >>
+  let+ new_queueA := (SwapBackD queue outD) in
+  match QueueFrontA new_queueA, outD with
+  (*Queue was empty - return the empty queue*)
+  | [], _ => Tick.ret new_queueA
+  (*Queue was non-empty - push the value back on the queue*)
+  | _, Some (xA, queueA) => Tick.ret (Thunk (appendD xA (QueueBackA new_queueA)))
+  (*Can't happen - will never have a non-empty list and an empty demand*)
+  | h1 :: t1, _ => bottom
+  end.
 
 (** Tests! **)
 
@@ -107,12 +131,22 @@ Compute Push_TwoListQueueD (TwoListQueue [] []) 4 (TwoListQueueA ((exact [])) (e
 
 (** Proofs! **)
 
+Lemma push_cost {a} (queue : two_list_queue a) (appending : a) (outD : two_list_queueA a)
+  : outD `is_approx` (Push_TwoListQueue queue appending) ->
+  Tick.cost (Push_TwoListQueueD queue appending outD) = 1.
+Proof.
+  auto.
+Qed.
+
 (*
 
 To prove:
-- Push is constant time; state and prove it.
+Done! Push is constant time; state and prove it.
+- Pop first, then computation costs about it.
 - If I finish it, think about best way to prove functional correctness.
   - Equivalence to pure version?
     - Prove that the pure version is also correct by showing that it's equal to a *lesser* queue using just one list
+  - Input demand leq the input of the pure version + (fun xs = zs, fun xs zsD = xsD, zs `is_approx` zsD) -> (xsD `is_approx` xs)
+  - At some point, define the approx function PushTLQA and prove equivalence with PushTLQD.
 
 *)
